progress on generic online softmax lemma

src/lib/math/Kuiper.Math.OnlineSoftmax.fst
@@ -5,13 +5,25 @@ open Kuiper
 open Kuiper.Spec.Softmax
 open Kuiper.Seq.Common
 
-let exp_sum (s : seq real{len s > 0}) : r:real{r >. 0.0R} =
-  rsum (seq_map rexp s)
+// NB: this file follows naming conventions of the 
+// original online softmax paper, whenever possible: https://arxiv.org/pdf/1805.02867
+// s = sequence (generic)
+// x = softmax input (sequence)
+// xi = some element of x
+// y = softmax output (sequence)
+// yi = some element of y
+// m = running max of x
+// d = running denominator sum of x
+// fxi = exp(xi-m) (actually from flash attention paper)
 
-let adjust_factor (s : seq real{len s > 0}) (x : real) : real =
-  exp_sum s
+
+let exp_sum (x : seq real{len x > 0}) : r:real{r >. 0.0R} =
+  rsum (seq_map rexp x)
+
+let adjust_factor (x : seq real{len x > 0}) (xi : real) : real =
+  exp_sum x
   /.
-  (exp_sum s +. rexp x)
+  (exp_sum x +. rexp xi)
 
 let rec seq_max (s : seq real{len s > 0})
   : Tot real (decreases len s)
@@ -21,58 +33,65 @@ let rec seq_max (s : seq real{len s > 0})
   | SNil -> h
   | SCons _ _ -> rmax h (seq_max t)
 
-let rec seq_max_cons_lem (s : seq real{len s > 0}) (x : real)
-  : Lemma (ensures seq_max (s @+ seq![x]) == rmax x (seq_max s))
+let rec seq_max_cons_lem (s : seq real{len s > 0}) (si : real)
+  : Lemma (ensures seq_max (s @+ seq![si]) == rmax si (seq_max s))
           (decreases len s)
-          [SMTPat (seq_max (s @+ seq![x]))]
+          [SMTPat (seq_max (s @+ seq![si]))]
   = let SCons h t = view_seq s in
-    assert Seq.equal (s @+ seq![x]) (Seq.cons h (t @+ seq![x]));
+    assert Seq.equal (s @+ seq![si]) (Seq.cons h (t @+ seq![si]));
     match view_seq t with
     | SNil ->
-      lem_rmax_comm x (seq_max s)
+      lem_rmax_comm si (seq_max s)
     | SCons _ _ ->
       calc (==) {
-        seq_max (s @+ seq![x]);
+        seq_max (s @+ seq![si]);
         == {}
-        rmax h (seq_max (t @+ seq![x]));
-        == { seq_max_cons_lem t x }
-        rmax h (rmax x (seq_max t));
-        == { lem_rmax_assoc h x (seq_max t)}
-        rmax (rmax h x) (seq_max t);
-        == {}
-        rmax x (seq_max s);
+        rmax h (seq_max (t @+ seq![si]));
+        == { seq_max_cons_lem t si }
+        rmax h (rmax si (seq_max t));
+        == { lem_rmax_assoc h si (seq_max t)}
+        rmax (rmax h si) (seq_max t);
+        //== { lem_rmax_comm h si }
+        //rmax (rmax si h) (seq_max t);
+        //== { lem_rmax_assoc si h (seq_max t) }
+        //rmax si (rmax h (seq_max t));
+        == { }
+        rmax si (seq_max s);
       }
 
 // should not restrict len s > 0 eventually,
 // but the initial state makes things weird
 noeq
-type st (s : erased (seq real){len s > 0}) = {
+type st (x : erased (seq real){len x > 0}) = {
   m : real; // maximum so far
   d : real; // denominator, i.e. the sum of exponentials, corrected
-  #m_ok : m == seq_max s;
-  #d_ok : d >. 0.0R /\ d == exp_sum s /. rexp m;
+  #m_ok : m == seq_max x;
+  #d_ok : d >. 0.0R /\ d == exp_sum x /. rexp m;
 }
 
-let exp_sum_snoc_lem (s : seq real{len s > 0}) (x : real)
-  : Lemma (exp_sum (s @+ seq![x]) == exp_sum s +. rexp x)
+let exp_sum_snoc_lem (x : seq real{len x > 0}) (xi : real)
+  : Lemma (exp_sum (x @+ seq![xi]) == exp_sum x +. rexp xi)
   = calc (==) {
-    exp_sum (s @+ seq![x]);
+    exp_sum (x @+ seq![xi]);
     == {}
-    rsum (seq_map rexp (s @+ seq![x]));
+    rsum (seq_map rexp (x @+ seq![xi]));
     == {}
-    rsum (seq_map rexp s) +. rsum (seq_map rexp (seq![x]));
+    rsum (seq_map rexp x) +. rsum (seq_map rexp (seq![xi]));
     == {}
-    exp_sum s +. rexp x;
+    exp_sum x +. rexp xi;
   }
 
 let r_distr_r (a b c : real) : Lemma (a *. (b +. c) == a *. b +. a *. c) = ()
 let r_distr_l (a b c : real{c =!= 0.0R}) : Lemma ((a +. b) /. c == a /. c +. b /. c) = ()
 
-let cancel (a : real) (b : real{b =!= 0.0R}) : Lemma (a *. b /. b == a) = ()
+let cancel_md (a : real) (b : real{b =!= 0.0R}) : Lemma (a *. b /. b == a) = ()
+let cancel_dm (a : real) (b : real{b =!= 0.0R}) : Lemma (a /. b *. b == a) = ()
 let abcd_adcb (a b c d : real{b =!= 0.0R /\ d =!= 0.0R})
   : Lemma (a /. b *. c /. d == a /. d *. c /. b) = ()
 
-let cancel' (a b c : real{b =!= 0.0R /\ c =!= 0.0R}) : Lemma ((a /. c) /. (b /. c) == a /. b) =
+let assoc_mul (a b c: real) : Lemma ((a *. b) *. c == a *. (b *. c)) = ()
+
+let cancel_ddd (a b c : real{b =!= 0.0R /\ c =!= 0.0R}) : Lemma ((a /. c) /. (b /. c) == a /. b) =
   calc (==) {
     (a /. c) /. (b /. c);
     == {}
@@ -86,50 +105,223 @@ let assoc_mul_div (a b c : real{c =!= 0.0R}) : Lemma ((a *. b) /. c == a *. (b /
 
 #push-options "--split_queries always --z3rlimit 5 --retry 5" // very bad smt performance below
 #restart-solver
-let softmax_step #s (s0 : st s) (x : real) :
-  res:(real & st (s @+ seq![x]))
-   { fst res /. (snd res).d == softmax_real (s @+ seq![x]) @! len s }
+let softmax_step #x (xst : st x) (xi : real) :
+  res:(real & st (x @+ seq![xi]) & real)
+   { (let (fxi,xst',adj) = res in
+    fxi /. xst'.d == softmax_real (x @+ seq![xi]) @! len x /\
+    adj == rexp (xst.m -. xst'.m)) }
   =
-  let m' = rmax s0.m x in
-  seq_max_cons_lem s x;
-  assert m' == seq_max (s @+ seq![x]);
-  let y = rexp (x -. m') in
-  exp_sum_snoc_lem s x;
-  assert s0.d == exp_sum s /. rexp s0.m;
-  let d' = s0.d *. rexp (s0.m -. m') +. y in
+  admit ();
+  let m' = rmax xst.m xi in
+  seq_max_cons_lem x xi;
+  assert m' == seq_max (x @+ seq![xi]);
+  let fxi = rexp (xi -. m') in
+  let adj = rexp (xst.m -. m') in
+  exp_sum_snoc_lem x xi;
+  assert xst.d == exp_sum x /. rexp xst.m;
+  let d' = xst.d *. adj +. fxi in
   assert (d' >. 0.0R);
   (* Prove d' is correct. *)
   calc (==) {
-    exp_sum (s @+ seq![x]) /. rexp m';
+    exp_sum (x @+ seq![xi]) /. rexp m';
     == {}
-    (exp_sum s +. rexp x) /. rexp m';
-    == { r_distr_l (exp_sum s) (rexp x) (rexp m') }
-    exp_sum s /. rexp m' +. rexp x /. rexp m';
-    == { cancel (exp_sum s /. rexp m') (rexp s0.m) }
-    exp_sum s /. rexp m' *. rexp s0.m /. rexp s0.m +. rexp x /. rexp m';
-    == { abcd_adcb (exp_sum s) (rexp s0.m) (rexp s0.m) (rexp m') }
-    exp_sum s /. rexp s0.m *. rexp s0.m /. rexp m' +. rexp x /. rexp m';
-    == { assoc_mul_div (exp_sum s /. rexp s0.m) (rexp s0.m) (rexp m') }
-    exp_sum s /. rexp s0.m *. (rexp s0.m /. rexp m') +. rexp x /. rexp m';
-    == { exp_sub s0.m m' }
-    exp_sum s /. rexp s0.m *. rexp (s0.m -. m') +. rexp x /. rexp m';
+    (exp_sum x +. rexp xi) /. rexp m';
+    == { r_distr_l (exp_sum x) (rexp xi) (rexp m') }
+    exp_sum x /. rexp m' +. rexp xi /. rexp m';
+    == { cancel_md (exp_sum x /. rexp m') (rexp xst.m) }
+    exp_sum x /. rexp m' *. rexp xst.m /. rexp xst.m +. rexp xi /. rexp m';
+    == { abcd_adcb (exp_sum x) (rexp xst.m) (rexp xst.m) (rexp m') }
+    exp_sum x /. rexp xst.m *. rexp xst.m /. rexp m' +. rexp xi /. rexp m';
+    == { assoc_mul_div (exp_sum x /. rexp xst.m) (rexp xst.m) (rexp m') }
+    exp_sum x /. rexp xst.m *. (rexp xst.m /. rexp m') +. rexp xi /. rexp m';
+    == { exp_sub xst.m m' }
+    exp_sum x /. rexp xst.m *. rexp (xst.m -. m') +. rexp xi /. rexp m';
     == {}
-    s0.d *. rexp (s0.m -. m') +. rexp x /. rexp m';
+    xst.d *. adj +. rexp xi /. rexp m';
     == { () }
     d';
   };
   (* Prove result is correct. *)
   calc (==) {
-    y /. d';
+    fxi /. d';
     == {}
-    rexp (x -. m') /. (exp_sum (s @+ seq![x]) /. rexp m');
+    rexp (xi -. m') /. (exp_sum (x @+ seq![xi]) /. rexp m');
     == {}
-    (rexp x /. rexp m') /. (exp_sum (s @+ seq![x]) /. rexp m');
-    == { cancel' (rexp x) (exp_sum (s @+ seq![x])) (rexp m') }
-    rexp x  /. exp_sum (s @+ seq![x]);
+    (rexp xi /. rexp m') /. (exp_sum (x @+ seq![xi]) /. rexp m');
+    == { cancel_ddd (rexp xi) (exp_sum (x @+ seq![xi])) (rexp m') }
+    rexp xi  /. exp_sum (x @+ seq![xi]);
     == {}
-    softmax_real (s @+ seq![x]) @! len s;
+    softmax_real (x @+ seq![xi]) @! len x;
   };
-  assert (y /. d' == softmax_real (s @+ seq![x]) @! len s);
-  y, { m=m'; d=d' }
+  assert (fxi /. d' == softmax_real (x @+ seq![xi]) @! len x);
+  fxi, { m=m'; d=d' }, adj
 #pop-options
+
+#push-options "--split_queries always --z3rlimit 10"
+let softmax_stepi (#n:pos) (x : lseq real n) (i: pos{i < n}) (xst : st (seq_take i x)) :
+  res:(real & st (seq_take (i+1) x) & real)
+   { (let (fxi,xst',adj) = res in
+    fxi /. xst'.d == softmax_real (seq_take (i+1) x) @! (len (seq_take i x)) /\
+    (i == (len (seq_take i x))) /\ // TODO shouldnt be necessary 
+    adj == rexp (xst.m -. xst'.m)) } = admit ()
+
+open Kuiper.DotProd
+
+#push-options "--split_queries always --z3rlimit 10"
+let lem_online_softmax_adj
+  (#n : pos)
+  (x : lseq real n)
+  (i: pos {i < n}) 
+  (xst : st (seq_take i x))
+  (k: real -> natlt (Seq.length x) -> real)  (* continuation: what to do with e^xi *)
+  (#k_comm_div: (nr: real) -> (dr: real { dr =!= 0.0R } ) -> (j: natlt n) -> (k nr j) /. dr == k (nr /. dr) j) 
+  (op: real -> real -> real)
+  (#op_distrib_mul: (a: real) -> (b: real) -> (r: real) -> (r *. a) `op` (r *. b) == r *. (a `op` b))
+  (init: real)
+  (#r : real):
+  (* TODO: get rid of the extra constraint here. The lemma still holds when k = 0, but we just can't call softmax_real on an empty sequence
+    (seq_take 0 z) because that would entail dividing by 0. *)
+  (* maybe it just needs to be a "softmax_real_safe" that returns an empty sequence given an empty sequence as input.
+    Because it would also not be possible to have the invariant below hold before the loop (when k = 0) on the client side code. *)
+  Lemma 
+        (requires r /. xst.d == (seq_fold_left op init (seq_mapi (softmax_real (seq_take i x)) k)))
+        (ensures 
+          (let (fxi,xst',adj) = softmax_stepi #n x i xst in
+          (r *. adj `op` (k fxi i)) /. xst'.d == (seq_fold_left op init (seq_mapi (softmax_real (seq_take (i+1) x)) k)))) =
+  
+    let (fxi,xst',adj) = softmax_stepi #n x i xst in
+
+    (*calc (==) {
+       (k fxi i /. xst'.d);
+       == { k_comm_div fxi xst'.d i }
+       (k (fxi /. xst'.d) i);
+       == {}
+       (k (softmax_real (seq_take (i+1) x) @! i) i);
+    };*)
+    
+    assert (rexp (xst.m -. xst'.m) == rexp (xst.m) /. rexp (xst'.m));
+
+    let x_upto_i = seq_take i x in
+    let x_upto_i' = seq_take (i+1) x in
+    let v1 = (seq_fold_left op init (seq_mapi (softmax_real (x_upto_i)) k)) in
+    calc (==) {
+      r *. adj /. xst'.d;
+      == { assoc_mul_div r adj xst'.d }
+      r *. (adj /. xst'.d);
+      == {}
+      r *. (rexp (xst.m) /. rexp (xst'.m) /. xst'.d);
+      == {}
+      r *. (rexp (xst.m) /. rexp (xst'.m) /. (exp_sum x_upto_i' /. (rexp xst'.m)));
+      == { cancel_ddd (rexp xst.m) (exp_sum x_upto_i') (rexp xst'.m)}
+      r *. (rexp (xst.m) /. (exp_sum x_upto_i'));
+      == { cancel_dm r xst.d }
+      v1 *. xst.d *. (rexp (xst.m) /. (exp_sum x_upto_i'));
+      == { assoc_mul v1 xst.d (rexp (xst.m) /. (exp_sum x_upto_i')) }
+      v1 *. (xst.d *. (rexp (xst.m) /. (exp_sum x_upto_i')));
+      == { }
+      v1 *. ((exp_sum x_upto_i /. (rexp xst.m)) *. (rexp (xst.m) /. (exp_sum x_upto_i')));
+      == { assoc_mul_div (exp_sum x_upto_i /. (rexp xst.m)) (rexp xst.m) (exp_sum x_upto_i') }
+      v1 *. (((exp_sum x_upto_i /. (rexp xst.m)) *. rexp (xst.m)) /. (exp_sum x_upto_i'));
+      == { cancel_dm (exp_sum x_upto_i) (rexp xst.m) }
+      v1 *. ((exp_sum x_upto_i) /. (exp_sum x_upto_i'));
+    };
+
+    // assume (forall (a b: real) (r: real { r =!= 0.0R }). (a /. r) `op` (b /. r) == (a `op` b) /. r); // TODO probably provable from above
+
+    admit ()
+(*
+
+let rec aux (#n : pos) (x y : lseq real n)  (#i : pos{i <= n})
+    (state : st (seq_take i x))
+    (r : real{r /. state.d == seq_dotprod' (softmax_real x) y i})
+    : Tot (r:real{r == seq_dotprod (softmax_real x) y})
+          (decreases n-i)
+  = let _ = if i = n
+    then (
+      r /. state.d
+    ) else (
+      let fx, state', _ = softmax_step state (x @! i) in
+      let adj = rexp (state.m -. state'.m) in
+      let r' = r *. adj   +.   fx *. (y @! i) in
+      let z = fx *. (y @! i) in
+      let tx = seq_take i x in 
+      assume Seq.equal (seq_take (i+1) x) (seq_take i x @+ seq![x @! i]); // seems ok...
+      let state' : st (seq_take (i+1) x) = coerce_eq () state' in
+      assert (len tx == i);
+      assert (fx /. state'.d == (softmax_real (tx @+ seq![x @! i])) @! i);
+      assert (fx /. state'.d == (softmax_real (seq_take (i+1) x)) @! i);
+      assert ((fx /. state'.d) *. (y @! i) == (softmax_real (seq_take (i+1) x) @! i) *. (y @! i));
+      assume ((fx /. state'.d) *. (y @! i) == z /. state'.d); // ???
+      
+      assert (rexp (state.m -. state'.m) == rexp (state.m) /. rexp (state'.m));
+      assume (r == seq_dotprod' (softmax_real x) y i *. state.d ); // ???
+      calc (==) {
+        (r *. adj /. state'.d);
+        == {}
+        ((seq_dotprod' (softmax_real x) y i) *. state.d *. adj /. state'.d);
+        == {}
+        ((seq_dotprod' (softmax_real x) y i) *. (exp_sum (seq_take i x) /. rexp state.m) *. adj /. (exp_sum (seq_take (i+1) x) /. rexp state'.m));
+        == {}
+        ((seq_dotprod' (softmax_real x) y i) *. (exp_sum (seq_take i x) /. exp_sum (seq_take (i+1) x)) *. (rexp state'.m /. rexp state.m) *. adj);
+        == {} 
+        ((seq_dotprod' (softmax_real x) y i) *. (exp_sum (seq_take i x) /. exp_sum (seq_take (i+1) x)));      
+      };
+      admit ();
+
+      calc (==) {
+        (r' /. state'.d);
+        == {}
+        (r *. adj +. fx *. (y @! i)) /. state'.d;
+        == {}
+        (r *. adj /. state'.d +. fx *. (y @! i) /. state'.d);
+        == {}
+        (r *. adj /. state'.d +. (softmax_real (seq_take (i+1) x) @! i) *. (y @! i));
+        == {}
+        ((seq_dotprod' (softmax_real x) y i) *. (exp_sum (seq_take i x) /. exp_sum (seq_take (i+1) x)) 
+          +. (softmax_real (seq_take (i+1) x) @! i) *. (y @! i));
+        // multiple non-trivial steps: the sum i cancels with seq_dotprod' (softmax_real ...), 
+        // then we get the correct sum of i+1, then we add the ith element
+        == { admit () } 
+        ((seq_dotprod' (softmax_real x) y (i+1)));
+      };
+      admit ();
+      
+      assert (r /. state.d == seq_dotprod' (softmax_real x) y i);
+      assert (r' /. state'.d == seq_dotprod' (softmax_real x) y (i+1));
+      aux #(n) x y #(i+1) state' r'
+    ) in 
+    magic ()
+*)
+
+(*
+#set-options "--split_queries always --z3rlimit 15"
+let softmax_dotprod (#n : pos) (x y : lseq real n) : r:real{r == seq_dotprod (softmax_real x) y} =
+  let rec aux (#i : pos{i <= n})
+    (state : st (seq_take i x))
+    (r : real{r /. state.d == seq_dotprod' (softmax_real x) y i})
+    : Tot (r:real{r == seq_dotprod (softmax_real x) y})
+          (decreases n-i)
+  =
+    let _ = if i = n
+    then (
+      r /. state.d
+    ) else (
+      let fx, state', _ = softmax_step state (x @! i) in
+      let adj = rexp (state.m -. state'.m) in
+      let r' = r *. adj   +.   fx *. (y @! i) in
+      let z = fx *. (y @! i) in
+      assert (seq_take (i+1) x == seq_take i x @+ seq![x @! i]);
+      admit();
+      assert (z /. state'.d == (softmax_real (seq_take (i+1) x) @! i) *. (y @! i));
+      assume Seq.equal (seq_take (i+1) x) (seq_take i x @+ seq![x @! i]); // seems ok...
+      let state' : st (seq_take (i+1) x) = coerce_eq () state' in
+      assert (r /. state.d == seq_dotprod' (softmax_real x) y i);
+      assert (r' /. state'.d == seq_dotprod' (softmax_real x) y (i+1));
+      aux #(i+1) state' r'
+    ) in
+    magic ()
+  in
+  admit();
+  let r : r:real{r == seq_dotprod (softmax_real x) y} = magic() in
+  let s : st (seq_take 1 x) = magic() in
+  aux s r *)
